Use concrete var nums for compile_file_get_sz
The older version failed during the proof term check with an OOM error.
Using predeclared variables instead of declarations allows the term to
compile, but doesn't solve the actual problem.

src/Extract/ExtractAsyncFS.v
@@ -88,7 +88,49 @@ Ltac dbg_find_pre x:= match goal with
   end || idtac
 end.
 
-Example compile_file_get_sz : sigT (fun p => source_stmt p /\
+Fixpoint decls_pre (l : list Declaration) (n : nat) : pred :=
+  match l with
+  | [] => emp
+  | @Decl T Wr _ :: l0 => (n ~> zeroval ✶ decls_pre l0 (S n))%pred
+  end.
+
+Fixpoint decls_post (l : list Declaration) (n : nat) : pred :=
+  match l with
+  | [] => emp
+  | @Decl T Wr _ :: l0 => (n ~>? T * decls_post l0 (S n))%pred
+  end.
+
+Lemma decls_pre_impl_post :
+  forall decls n,
+    @decls_pre decls n =p=> decls_post decls n.
+Proof.
+  induction decls; intros.
+  - auto.
+  - destruct a.
+    cancel. auto.
+Qed.
+Hint Resolve decls_pre_impl_post : cancel_go_finish.
+
+Hint Extern 0 (okToCancel (decls_pre ?decls ?n) (decls_post ?decls ?n)) =>
+  apply decls_pre_impl_post.
+
+Ltac do_declare T cont ::=
+  lazymatch goal with
+  | [ |- EXTRACT _ {{ ?pre }} _ {{ _ }} // _ ] =>
+    simpl decls_pre;
+    lazymatch goal with
+    | [ |- EXTRACT _ {{ ?pre }} _ {{ _ }} // _ ] =>
+      lazymatch pre with
+      | context [decls_pre ?decls ?n] =>
+        let decls' := fresh "decls" in
+        evar (decls' : list Declaration);
+        unify decls (Decl T :: decls'); subst decls';
+        cont (n)
+      end
+    end
+  end.
+
+Example compile_file_get_sz : sigT (fun p => source_stmt p /\ exists vars,
   forall env fsxp inum ams,
   prog_func_call_lemma
     {|
@@ -115,17 +157,20 @@ Example compile_file_get_sz : sigT (fun p => source_stmt p /\
   {{ 0 ~>? (bool * Log.LOG.memstate * (word 64 * unit)) *
      1 ~> fsxp *
      2 ~> inum *
-     3 ~> ams }}
+     3 ~> ams * decls_pre vars 4}}
     p
   {{ fun ret => 0 ~> ret *
      1 ~>? FSLayout.fs_xparams *
      2 ~>? addr *
-     3 ~>? BFile.BFILE.memstate }} // env).
+     3 ~>? BFile.BFILE.memstate * decls_post vars 4}} // env).
 Proof.
+
   unfold AFS.file_get_sz, AFS.MSLL, pair_args_helper, BFile.BFILE.MSAlloc, Inode.INODE.ABytes.
   change Log.LOG.commit_ro with Log.LOG.begin.
+  eexists. split. shelve. eexists.
+  intros.
   compile_step.
-  compile_step.
+
   compile_step.
   solve [repeat compile_step].
   compile_step.
@@ -191,12 +236,18 @@ match goal with
                            | cancel_go.. ])))
           end)
 end.
-  compile_split.
-  compile_join.
-  compile_join.
+  compile_step.
+  compile_step.
+Ltac cancel_go ::=
+  unfold var; cancel; try apply pimpl_refl.
+  compile_step.
+
+  Check "finished construction for compile_file_get_sz".
 Unshelve.
   all : compile.
+  Check "finished script for compile_file_get_sz".
 Defined.
+Check "Defined compile_file_get_sz".
 
 Eval lazy in (projT1 compile_file_get_sz).
 
